src/TicketLock.v
@@ -81,18 +81,114 @@ From Fairness Require Import IProp IPM Weakest.
 From Fairness Require Import ModSim PCM MonotonePCM ThreadsRA StateRA FairRA.
 
 
-
 Section SIM.
   Context `{Σ: GRA.t}.
+
+
+  Fixpoint list_prop_sum A (l: list A) (P: A -> iProp): iProp :=
+    match l with
+    | [] => True
+    | hd::tl => P hd ** list_prop_sum tl P
+    end.
+
+  Lemma list_prop_sum_perm A (l0 l1: list A) P
+        (PERM: Permutation l0 l1)
+    :
+    list_prop_sum l0 P ⊢ list_prop_sum l1 P.
+  Proof.
+    induction PERM; ss.
+    { iIntros "[H0 H1]". iFrame. iApply IHPERM. auto. }
+    { iIntros "[H0 [H1 H2]]". iFrame. }
+    { etrans; eauto. }
+  Qed.
+
+  Definition natmap_prop_sum A (f: NatMap.t A) (P: nat -> A -> iProp) :=
+    list_prop_sum (NatMap.elements f) (fun '(k, v) => P k v).
+
+  Lemma natmap_prop_sum_empty A P
+    :
+    ⊢ natmap_prop_sum (NatMap.empty A) P.
+  Proof.
+    unfold natmap_prop_sum. ss. auto.
+  Qed.
+
+  Lemma natmap_prop_remove_find A (f: NatMap.t A) P k v
+        (FIND: NatMap.find k f = Some v)
+    :
+    (natmap_prop_sum f P)
+      -∗
+      (P k v ** natmap_prop_sum (NatMap.remove k f) P).
+  Proof.
+    hexploit NatMap.elements_1.
+    { eapply NatMap.find_2; eauto. }
+    i. eapply SetoidList.InA_split in H. des.
+    destruct y. inv H. ss. subst.
+    unfold natmap_prop_sum. rewrite H0.
+    iIntros "H".
+    iPoseProof (list_prop_sum_perm with "H") as "H".
+    { instantiate (1:=(k0,a)::(l1 ++ l2)).
+      symmetry. apply Permutation_middle.
+    }
+    iEval (ss) in "H". iDestruct "H" as "[H0 H1]". iFrame.
+    iApply (list_prop_sum_perm with "H1").
+    symmetry. eapply Permutation_remove.
+    rewrite H0. symmetry. apply Permutation_middle.
+  Qed.
+
+  Lemma natmap_prop_remove A (f: NatMap.t A) P k
+    :
+    (natmap_prop_sum f P)
+      -∗
+      (natmap_prop_sum (NatMap.remove k f) P).
+  Proof.
+    destruct (NatMap.find k f) eqn:EQ.
+    { iIntros "H". iPoseProof (natmap_prop_remove_find with "H") as "[_ H]"; eauto. }
+    replace (NatMap.remove k f) with f; auto.
+    eapply eq_ext_is_eq. ii.
+    rewrite NatMapP.F.remove_mapsto_iff. split.
+    { i. split; auto. ii.
+      eapply NatMap.find_1 in H. clarify.
+    }
+    { i. des. auto. }
+  Qed.
+
+  Lemma natmap_prop_sum_add A P k v (f: NatMap.t A)
+    :
+    (natmap_prop_sum f P)
+      -∗
+      (P k v)
+      -∗
+      (natmap_prop_sum (NatMap.add k v f) P).
+  Proof.
+    destruct (NatMapP.F.In_dec f k).
+    { rewrite <- nm_add_rm_eq. iIntros "H0 H1".
+      unfold natmap_prop_sum.
+      iApply list_prop_sum_perm.
+      { symmetry. eapply Permutation_add; eauto. apply NatMap.remove_1; auto. }
+      iPoseProof (natmap_prop_remove with "H0") as "H0".
+      ss. iFrame.
+    }
+    { unfold natmap_prop_sum. iIntros "H0 H1".
+      iApply list_prop_sum_perm.
+      { symmetry. eapply Permutation_add; eauto. }
+      ss. iFrame.
+    }
+  Qed.
+
   Context `{EXCL: @GRA.inG (Excl.t unit) Σ}.
   Context `{MONORA: @GRA.inG monoRA Σ}.
   Context `{THSRA: @GRA.inG ths_RA Σ}.
-  (* Context `{STATESRC: @GRA.inG (stateSrcRA unit) Σ}. *)
+  Context `{STATESRC: @GRA.inG (stateSrcRA (bool * NatMap.t unit)) Σ}.
   Context `{STATETGT: @GRA.inG (stateTgtRA (unit * SCMem.t)) Σ}.
   Context `{IDENTSRC: @GRA.inG (identSrcRA (id_sum thread_id void) (mk_wf Ord.lt_well_founded)) Σ}.
-  (* Context `{IDENTTGT: @GRA.inG (identTgtRA (void + SCMem.pointer)%type) Σ}. *)
+  Context `{IDENTTGT: @GRA.inG (identTgtRA (id_sum void SCMem.val)) Σ}.
   (* Context `{IDENTTHS: @GRA.inG identThsRA Σ}. *)
   Context `{MEMRA: @GRA.inG memRA Σ}.
+  Context `{FAIRSRC: @GRA.inG (@FairRA.t thread_id Ord.t _) Σ}.
+  (* Context `{IDENTTGT: @GRA.inG (identTgtRA ident_tgt) Σ}. *)
+
+
+
 
   Global Program Instance ge_PreOrder: PreOrder ge.
   Next Obligation.
@@ -153,10 +249,10 @@ Section SIM.
     { ii. unfold partial_map_singleton, partial_map_update in *. des_ifs. }
   Qed.
 
-  Fixpoint waiters now_serving (n: nat): iProp :=
+  Fixpoint waiters now_serving (n: nat) (W: NatMap.t unit): iProp :=
     match n with
     | 0 => True
-    | S n => (∃ i, (monoWhite 1 (@partial_map_PreOrder nat nat) (partial_map_singleton (now_serving + n) i)) ** Pending i) ** (waiters now_serving n)
+    | S n' => (∃ i, (monoWhite 1 (@partial_map_PreOrder nat nat) (partial_map_singleton (now_serving + n) i)) ** Pending i ** natmap_prop_sum W (fun k _ => FairRA.white k (Ord.S Ord.O))) ** (waiters now_serving n' W)
     end.
 
   Let I: iProp :=
@@ -165,11 +261,12 @@ Section SIM.
               **
               (St_tgt (tt, m)))
           **
-          (∃ im0 im1 (W: NatMap.t unit) (b: bool),
-              (OwnM (Auth.white (Excl.just (imap_sum_id (im0, im1)): @Excl.t _): identSrcRA (id_sum thread_id void) (mk_wf Ord.lt_well_founded)))
+          (∃ (im: imap thread_id (mk_wf Ord.lt_well_founded)) im_void,
+              (FairRA.blacks im)
                 **
-                (St_src void (W, b)))
+              (OwnM (Auth.white (Excl.just (imap_sum_id (im, im_void)): @Excl.t _): identSrcRA (id_sum thread_id void) (mk_wf Ord.lt_well_founded))))
           **
+
           (∃ now_serving n,
               (points_to TicketLock.next_ticket (SCMem.val_nat (now_serving + n)))
                 **
@@ -177,21 +274,91 @@ Section SIM.
                 **
                 (monoBlack 0 ge_PreOrder now_serving)
                 **
-                (waiters now_serving n)
-                **
                 (∃ f,
                     (monoBlack 1 (@partial_map_PreOrder nat nat) f)
                       **
                       (⌜forall m (LT: now_serving + n < m), f m = None⌝))
                 **
-                (∃ i,
-                    (monoWhite 1 (@partial_map_PreOrder nat nat) (partial_map_singleton now_serving i))
-                      **
-                      (Eventually i (points_to TicketLock.now_serving (SCMem.val_nat now_serving))))
-)
-  .
+                ((⌜n = 0⌝ ** St_src (false, NatMap.empty unit))
+                 ∨
+                   (∃ n', ⌜n = S n'⌝ ** ∃ W, St_src (false, W) ** waiters now_serving n' W))).
 
+  Definition blacks_success_single (tid: thread_id) (o: Ord.t)
+             (f0: imap thread_id (mk_wf Ord.lt_well_founded))
+    :
+    (FairRA.blacks f0)
+      -∗
+      (#=>
+         (∃ (f1: imap thread_id (mk_wf Ord.lt_well_founded)),
+             ((FairRA.blacks f1)
+                **
+                (FairRA.white tid o)
+                **
+                ⌜fair_update f0 f1 (fun i => if tid_dec i tid then Flag.success else Flag.emp)⌝))).
+  Admitted.
 
+  Definition blacks_fail_single (tid: thread_id)
+             (f0: imap thread_id (mk_wf Ord.lt_well_founded))
+    :
+    (FairRA.blacks f0)
+      -∗
+      (FairRA.white tid (Ord.S Ord.O))
+      -∗
+      (#=>
+         (∃ (f1: imap thread_id (mk_wf Ord.lt_well_founded)),
+             ((FairRA.blacks f1)
+                **
+                ⌜fair_update f0 f1 (fun i => if tid_dec i tid then Flag.fail else Flag.emp)⌝))).
+  Admitted.
+
+  Lemma imap_sum_update_l (A B: ID) (W: WF)
+        (im_l0 im_l1: imap A W) (im_r: imap B W) fm
+        (UPD: fair_update im_l0 im_l1 fm)
+    :
+    fair_update
+      (imap_sum_id (im_l0, im_r))
+      (imap_sum_id (im_l1, im_r))
+      (sum_fmap_l fm).
+  Proof.
+    ii. unfold sum_fmap_l. des_ifs.
+    { specialize (UPD a). des_ifs. }
+    { specialize (UPD a). des_ifs. }
+  Qed.
+
+  Lemma imap_sum_update_r (A B: ID) (W: WF)
+        (im_l: imap A W) (im_r0 im_r1: imap B W) fm
+        (UPD: fair_update im_r0 im_r1 fm)
+    :
+    fair_update
+      (imap_sum_id (im_l, im_r0))
+      (imap_sum_id (im_l, im_r1))
+      (sum_fmap_r fm).
+  Proof.
+    ii. unfold sum_fmap_r. des_ifs.
+    { specialize (UPD b). des_ifs. }
+    { specialize (UPD b). des_ifs. }
+  Qed.
+
+  Lemma fair_white_eq k o0 o1
+        (EQ: Ord.eq o0 o1)
+    :
+    (FairRA.white k o0)
+      -∗
+      (FairRA.white k o1).
+  Proof.
+    erewrite FairRA.white_eq; eauto.
+  Qed.
+
+  Lemma fair_white_one k o
+    :
+    (FairRA.white k (Ord.S o))
+      -∗
+      (FairRA.white k o ** FairRA.white k (Ord.S Ord.O)).
+  Proof.
+    iIntros "H". iApply FairRA.white_split. ss.
+    iApply (fair_white_eq with "H").
+    erewrite Hessenberg.add_S_r. rewrite Hessenberg.add_O_r. reflexivity.
+  Qed.
 
   Lemma sim: ModSim.mod_sim TicketLock.mod FairLock.mod.
   Proof.
@@ -209,13 +376,107 @@ Section SIM.
         destruct (Any.downcast args); ss.
         2:{ unfold UB. lred. iApply fsim_UB. }
         lred. rred. rewrite close_itree_call. ss. rred.
-        iApply (@fsim_sync _ _ _ _ _ _ _ None). ss. iFrame. iIntros "INV _".
-        rred. unfold SCMem.cas_fun, Mod.wrap_fun. rred.
-        lred. iApply fsim_tidL. lred.
-        iDestruct "INV" as "[[[%m [MEM ST]] SRC] [% [% [% [% [NEXT TK]]]]]]".
+        iApply fsim_sync. instantiate (1:=None). ss. iFrame. iIntros "INV _".
+        rred. lred. iApply fsim_tidL. lred.
+        iDestruct "INV" as "[[[%m [MEM TGT]] IM] [% [% [[[[NEXT NOW] MONO] MAP] WAIT]]]]".
+        unfold Mod.wrap_fun, SCMem.faa_fun.
         rred. iApply fsim_getR. iSplit.
         { iFrame. }
         rred. iApply fsim_tauR.
+        iPoseProof (memory_ra_faa with "MEM NEXT") as "[% [% > [MEM NEXT]]]".
+        rred. rewrite H.
+        rred. iApply fsim_getR. iSplit.
+        { iFrame. }
+        rred. iApply (fsim_putR with "TGT"). iIntros "TGT".
+        rred. iApply fsim_tauR.
+        rred. iApply fsim_tauR.
+        iPoseProof "IM" as "[% [% [BLACK IM]]]".
+        rred. iDestruct "WAIT" as "[[% SRC]|H]".
+        { subst. iApply fsim_getL. iSplit.
+          { iFrame. }
+          lred. iApply (fsim_putL with "SRC"). iIntros "SRC".
+          iPoseProof ((@blacks_success_single tid (Ord.S (Ord.S Ord.O))) with "BLACK") as "> [% [[BLACK FUEL] %]]".
+          lred. iApply (fsim_fairL with "IM"). iExists _. iSplit.
+          { iPureIntro. eapply imap_sum_update_l; eauto. }
+          iIntros "IM".
+          iPoseProof (fair_white_one with "FUEL") as "[FUEL ONE]".
+          iApply fsim_alloc_obligation.
+          { instantiate (1:=Ord.S (Ord.S (Ord.O))).
+            iIntros "% PENDING NEG # POS".
+            iPoseProof "MAP" as "[% [MAP %]]".
+            iPoseProof (black_updatable with "MAP") as "> MAP".
+            { instantiate (1:=(fun m => if (Nat.eq_dec m (now_serving + 1)) then Some k else f m)).
+              ii. des_ifs. exfalso. rewrite H1 in SOME; ss. lia.
+            }
+
+
+tid_dec
+
+            iAssert (#=> (I ** monoBlack 1 (partial_map_PreOrder nat nat) (partial_map_singleton (now_serving + 1))) with "[NOW MONO MAP MEM NEXT TGT SRC BLACK IM FUEL ONE]" as "INV".
+            { unfold I. iSplitL "MEM TGT BLACK IM".
+              { iModIntro. iSplitL "MEM TGT".
+                { iExists _. iFrame. }
+                { iExists _, _. iFrame. }
+              }
+              iExists now_serving, 1. iFrame. iSplitL "NEXT MAP".
+              { monoBlack 1 (partial_map_PreOrder nat nat) (partial_map_singleton (now_serving + 1) )
+
+ss.
+
+, _. iFrame.
+
+
+ red.
+
+          rewrite unfold_iter_eq. lred. iApply fsim_chooseL. iExists true.
+          lred.
+
+(inl ).
+
+          rewrite ITree.iter
+
+          iPoseProof ((@blacks_success_single tid (Ord.S (Ord.S Ord.O))) with "IMBLACK") as "> [% [[IMBLACK FUEL] %]]".
+          lred. iApply (fsim_fairL with "IM"). iExists _. iSplit.
+          { iPureIntro. eapply imap_sum_update_l; eauto. }
+          iIntros "IM".
+
+
+
+blacks_fail_single
+          lred.
+
+          {
+
+
+          ss.
+          { ss. unfold OMod.closed_ident. ss. eapply IDENTTGT.
+unfold
+
+s
+
+          iPoseProof (memory_ra_faa with "MEM NEXT") as "[% [% > [MEM NEXT]]]".
+
+
+
+
+iApply fsim_tauR.
+
+iApply (fsim_putR with "ST"). iIntros "ST".
+
+iSplit.
+        { iFrame. }
+
+
+ss. des; clarify.
+
+
+        rred. iApply fsim_getR. iSplit.
+        { iFrame. }
+        rred. iApply fsim_tauR.
+        iPoseProof (memory_ra_load with "MEM NEXT") as "%". ss. des; clarify.
+        rred. ss. rewrite H.
+
+                iPoseProof (memory_ra_load
         rred.
 
 [% [% [% [% H]]]]]".
